# Even and Odd Functions

## Parity of Functions

 - $cos$ is an **even function**:
   - $\cos(-\alpha) = \cos(\alpha)$
   - therefore: $\cos(\alpha-\beta) = \cos(\beta-\alpha)$
- $sin$ and $tan$ are **odd functions**:
  - $\sin(-\alpha) = -\sin(\alpha)$
  - therefore: $\sin(\alpha-\beta) = -\sin(\beta-\alpha)$
  - $\tan(-\alpha) = -\tan(\alpha)$
  - therefore: $\tan(\alpha-\beta) = -\tan(\beta-\alpha)$

## Sum and Difference in Terms of Parity

### Sine/Cosine

$$
\begin{array}{l}
\left[\begin{array}{l}
\sin(x) \pm \cos(-x) = \sin(x) \pm \cos(x)
\\
\sin(-x) \pm \cos(-x) = \pm \cos(x) - \sin(x)
\\
\sin(-x) - \cos(x) = -\sin(x)-\cos(x)
\end{array}\right.
\\
\\
\left[\begin{array}{l}
\sin(\alpha) \pm \cos(-\beta) = \sin(\alpha) \pm \cos(\beta)
\\
\sin(-\alpha) \pm \cos(-\beta) = -\sin(\alpha) \pm \cos(\beta)
\\
\sin(-\alpha) - \cos(\beta) = -\sin(\alpha)-\cos(\beta)
\end{array}\right.
\end{array}
$$

### Cosine/Sine

$$
\begin{array}{l}
\left[\begin{array}{l}
\cos(x) \pm \sin(-x) = \cos(x) \mp \sin(x)
\\
\cos(-x) \pm \sin(-x) = \cos(x) \mp \sin(x)
\\
\cos(-x) - \sin(x) = \cos(x)-\sin(x)
\end{array}\right.
\\
\\
\left[\begin{array}{l}
\cos(\alpha) \pm \sin(-\beta) = \cos(\alpha) \mp \sin(\beta)
\\
\cos(-\alpha) \pm \sin(-\beta) = \cos(\alpha) \mp \sin(\beta)
\\
\cos(-\alpha) - \sin(\beta) = \cos(\alpha)-\sin(\beta)
\end{array}\right.
\end{array}
$$

### Sines

$$
\begin{array}{l}
\left[\begin{array}{l}
\sin(x) + \sin(-x) = 0
\\
\sin(\pm x) - \sin(\mp x) = 2\sin(\pm x)
\\
\sin(-x) \pm \sin(-x) = (-1 \mp 1)\sin(x)
\end{array}\right.
\\
\\
\left[\begin{array}{l}
\sin(\alpha) + \sin(-\beta) = \sin(\alpha) - \sin(\beta)
\\
\sin(\pm \alpha) - \sin(\mp \beta) = \pm \sin(\alpha) \pm \sin(\beta)
\\
\sin(-\alpha) \pm \sin(-\beta) = \mp \sin(\alpha) \mp \sin(\beta)
\end{array}\right.
\end{array}
$$

### Cosines

$$
\begin{array}{l}
\left[\begin{array}{l}
\cos(x) + \cos(-x) = 2\cos(x)
\\
\cos(\pm x) - \cos(\mp x) = 0
\\
\cos(-x) \pm \cos(-x) = (1 \pm 1)\cos(x)
\end{array}\right.
\\
\\
\left[\begin{array}{l}
\cos(\alpha) + \cos(-\beta) = \cos(\alpha) + \cos(\beta)
\\
\cos(\pm \alpha) - \cos(\mp \beta) = \cos(\alpha) - \cos(\beta)
\\
\cos(-\alpha) \pm \cos(-\beta) = \cos(\alpha) \pm \cos(\beta)
\end{array}\right.
\end{array}
$$
