# Sum/Difference of Trigonometric Functions and 1

$$
\begin{array}{rl}
1 \pm \sin(\theta) & = 2 \sin^2\left(
\frac{1}{4}\pi \pm \frac{1}{2}\theta
\right)
\\
\ 
\\
& = 2 \cos^2\left(
\frac{1}{4}\pi \mp \frac{1}{2}\theta
\right)
\\
\ 
\\
1+\cos(\theta) & = 2 \cos^2\left(\frac{1}{2}\theta\right)
\\
\ 
\\
1-\cos(\theta) & = 2 \sin^2\left(\frac{1}{2}\theta\right)
\\
\ 
\\
\ 
\end{array}
$$

> $f(\theta)-1 = -(1-f(\theta))$

## Squared Function

### Sine

$$
\begin{array}{rl}
1+\sin^2(\theta) & = 2-\cos^2(\theta)
\\
& = \frac{1}{2}(3-\cos(2\theta))
\\
\ 
\\
1-\sin^2(\theta) & = (1-\sin(\theta))(1+\sin(\theta))
\\
& = \cos^2(\theta)
\\
& = \frac{1}{2}(\cos(2\theta)+1)
\\
\ 
\\
\sin^2(\theta)-1 & = (\sin(\theta)-1)(\sin(\theta)+1)
\\
& = -\cos^2(\theta)
\\
& = -\frac{1}{2}(\cos(2\theta)+1)
\end{array}
$$

### Cosine

$$
\begin{array}{rl}
1+\cos^2(\theta) & = 2-\sin^2(\theta)
\\
& = \frac{1}{2}(3+\cos(2\theta))
\\
\ 
\\
1-\cos^2(\theta) & = (1-\cos(\theta))(1+\cos(\theta))
\\
& = \sin^2(\theta)
\\
& = \frac{1}{2}(1-\cos(2\theta))
\\
\ 
\\
\cos^2(\theta)-1 & = (\cos(\theta)-1)(\cos(\theta)+1)
\\
& = -\sin^2(\theta)
\\
& = \frac{1}{2}(\cos(2\theta)-1)
\end{array}
$$

### Definitions of the Squared Functions

$$
\begin{array}{rl}
\sin^2(\theta) & = \frac{1}{2}(1-\cos(2\theta))
\\
\ 
\\
& = 1-\cos^2(\theta)
\\
\ 
\\
& = \cos^2\left(
 \frac{1}{2}\pi-\theta
\right)
\\
\ 
\\
& = \frac{1}{\csc^2(\theta)}
\\
\ 
\\
\cos^2(\theta) & = \frac{1}{2}(1+\cos(2\theta))
\\
\ 
\\
& = 1-\sin^2(\theta)
\\
\ 
\\
& = \sin^2\left(
  \frac{1}{2}\pi-\theta
\right)
\\
\ 
\\
& = \frac{1}{\sec^2(\theta)}
\end{array}
$$

## Other Functions

$$
\begin{array}{rl}
1+\tan^2(\theta) & = \frac{1}{\cos^2(\theta)} = \sec^2(\theta)
\\
\ 
\\
1-\tan^2(\theta) & = (1-2\sin^2(\theta))\sec^2(\theta)
\\
\ 
\\
1+\cot^2(\theta) & = \frac{1}{\sin^2(\theta)} = \csc^2(\theta)
\\
\ 
\\
1-\cot^2(\theta) & = (2\sin^2(\theta)-1)\csc^2(\theta)
\\
\ 
\\
& = 2-\csc^2(\theta)
\end{array}
$$
