# Forms of Quadratic Functions

#### standard/general form:

$$
y = ax^2+bx+c
$$

#### vertex form:

$$
y = a(x-p)^2+q
$$

#### intercept/factored form:

$$
y = a(x-x_1)(x-x_2)
$$

$$
\text{or}
$$

$$
y = a(x-x_0)^2
$$

## Conversion

### From Standard Form

#### To Vertex Form

$$
\begin{array}{l}
ax^2+bx+c \quad \mapsto \quad a(x-p)^2+q
\\
\ 
\\
p = \frac{-b}{2a}
\\
q = c-ap^2
\end{array}
$$

#### To Intercept Form

$$
\begin{array}{l}
ax^2+bx+c \quad \mapsto \quad
a(x-x_1)(x-x_2)
\\
\ 
\\
x_{1,2} = \frac{-b\pm\sqrt{\Delta}}{2a}
\quad \iff \Delta \ge 0
\\
\Delta = b^2-4ac
\end{array}
$$

### From Vertex Form

#### To Standard Form

$$
\begin{array}{l}
a(x-p)^2+q \quad \mapsto \quad ax^2+bx+c
\\
\ 
\\
b = -2ap
\\
c = ap^2+q
\end{array}
$$

#### To Intercept Form

$$
\begin{array}{l}
a(x-p)^2+q \quad \mapsto \quad a(x-x_1)(x-x_2)
\\
\ 
\\
b = -2ap
\\
c = ap^2+q
\\
x_{1,2} = \frac{-b\pm\sqrt{\Delta}}{2a}
\quad \iff \Delta \ge 0
\\
\Delta = b^2-4ac
\end{array}
$$

### From Intercept Form

#### To Standard Form

$$
\begin{array}{l}
a(x-x_1)(x-x_2) \quad \mapsto \quad ax^2+bx+c
\\
\ 
\\
b = -a(x_1 + x_2)
\\
c = ax_1x_2
\end{array}
$$

#### To Vertex Form

$$
\begin{array}{l}
a(x-x_1)(x-x_2) \quad \mapsto \quad a(x-p)^2+q
\\
\ 
\\
p = \frac{x_1 + x_2}{2}
\\
q = -a(p-x_1)^2
\end{array}
$$
