# Properties of Logarithms

## Product/Quotient Property

$$
\begin{array}{l}
\log_n(ab) = \log_n(a) + \log_n(b)
\\
\log_n\left(\frac{a}{b}\right) = \log_n(a) - \log_n(b)
\end{array}
$$

## Power Property 

$$
\begin{array}{l}
\log_n(x^p) = p \log_n(x)
\\
\log_n(x^{pq}) = q \log_n(x^p) = pq \log_n(x)
\\
\ 
\\
\log_n(\sqrt[d]{x}) = \frac{1}{d} \log_n(x)
\\
\log_n(\sqrt[dt]{x}) = \frac{1}{t} \log_n(\sqrt[d]{x}) = \frac{1}{dt} \log_n(x)
\end{array}
$$

## Reciprocal Property

$$
\log_n(x) = \frac{1}{\log_x(n)}
$$

## Definition Property

$$
\log_n(x) = \frac{\ln(x)}{\ln(n)}
$$

## Base Change Property

$$
\log_n(x) = \log_n(k) \cdot \log_k(x)
$$

## Base Swap Property

$$
\begin{array}{rl}
\because & \log_a(b) \cdot \log_c(d) = \frac{
 \ln(b) \ln(d)
}{
 \ln(a) \ln(c)
}
\\
\therefore & \log_a(b) \cdot \log_c(d) = \log_c(b) \cdot \log_a(d)
\\
\ 
\\
\because & \frac{\log_a(b)}{\log_c(d)} = \frac{
 \ln(b) \ln(c)
}{
 \ln(a) \ln(d)
}
\\
\therefore & \frac{\log_a(b)}{\log_c(d)} = \log_a(c) \cdot \log_d(b)
\\
\ 
\\
\because & \log_a(b) = \frac{1}{\log_b(a)}
\\
\therefore & \frac{\log_a(b)}{\log_c(d)} = \log_a(b) \cdot \log_d(c)
\end{array}
$$

