# Summation

## Constant Multiplier

$$
\sum_{n=s}^t {\color{red}k}f(n) =
{\color{red}k} \sum_{n=s}^t f(n)
$$

$$
\sum_{n=s}^t \frac{f(n)}{{\color{red}k}} =
\frac{\displaystyle\sum_{n=s}^t f(n)}{{\color{red}{k}}}
$$

## Constant Summand

$$
\sum_{n=s}^t {\color{red}k} + f(n) =
(t-s+1){\color{red}k} +
\sum_{n=s}^t f(n)
$$

$$
\sum_{n=s}^t {\color{red}k} - f(n) =
(t-s+1){\color{red}k} -
\sum_{n=s}^t f(n)
$$

$$
\sum_{n=s}^t f(n) - {\color{red}k} =
\left[\sum_{n=s}^t f(n)\right] -
(t-s+1){\color{red}k}
$$




